Ballot/Ballot.v
@@ -1,6 +1,3 @@
-Require Import List.
-Require Import OrderedType.
-Require Import Coq.Program.Equality.
 Require Import Arith.
 Require Import Nat.
 Require Import OrderedTypeEx.
@@ -10,7 +7,26 @@ Require Import BinIntDef.
 Open Scope Z_scope.
 Include BinIntDef.Z.
 Module IntMap := FMapList.Make(Z_as_OT).
-Definition sender := 0.
+Definition contract_addr := 0.
+Definition EtherMap := IntMap.t Z.
+
+Definition get_ether (addr : Z) map : Z :=
+    match (IntMap.find addr map) with
+    | None => 0
+    | Some a => a
+    end.
+
+Definition send addr value map :=
+    if (Z.leb value (get_ether contract_addr map)) then
+        (let map_bis := IntMap.add contract_addr ((get_ether contract_addr map) - value) map in
+        let map_bis := IntMap.add addr ((get_ether addr map_bis) + value) map_bis in
+        (true, map_bis))
+    else (false, map).
+
+Record Message := create_message {
+sender : Z;
+value : Z;
+}.
 Record Ballot := create_Ballot { 
 voteCounts: IntMap.t (Z);
 delegations: IntMap.t (Z);
@@ -45,7 +61,7 @@ let m1:= match (IntMap.find a0 mapping)  with
  | None => 0
  | Some a => a end in 
 m1.
-Definition Ballot_constructor(_numProposals:Z)  := 
+Fixpoint Ballot_constructor(ether : EtherMap) (msg : Message)(_numProposals:Z)  := 
 let voteCounts := IntMap.empty (Z) in
 let delegations := IntMap.empty (Z) in
 let votes := IntMap.empty (Z) in
@@ -53,10 +69,11 @@ let voted := IntMap.empty (bool) in
 let voterWeight := IntMap.empty (Z) in
 let numProposals := 0 in
 let chairperson := 0 in
+let new_ether := ether in
 let chairperson := sender in 
 let numProposals := _numProposals in 
-(create_Ballot voteCounts delegations votes voted voterWeight numProposals chairperson).
-Definition giveRightToVote (Ballot:Ballot) (voter:Z)  := 
+((create_Ballot voteCounts delegations votes voted voterWeight numProposals chairperson), new_ether).
+Fixpoint giveRightToVote gas (Ballot:Ballot) (ether : EtherMap) (msg : Message)(voter:Z)  := 
 let voteCounts := (voteCounts Ballot) in
 let delegations := (delegations Ballot) in
 let votes := (votes Ballot) in
@@ -64,14 +81,17 @@ let voted := (voted Ballot) in
 let voterWeight := (voterWeight Ballot) in
 let numProposals := (numProposals Ballot) in
 let chairperson := (chairperson Ballot) in
-let Ballot2 := Ballot in 
-if ((get_voted voted  (voter))) then ((create_Ballot voteCounts delegations votes voted voterWeight numProposals chairperson)) 
+let new_ether := ether in 
+match gas with
+    | O => ((create_Ballot voteCounts delegations votes voted voterWeight numProposals chairperson), new_ether)
+ | S g => let new_gas := g in
+if ((get_voted voted  (voter))) then (((create_Ballot voteCounts delegations votes voted voterWeight numProposals chairperson), new_ether)) 
  else let imap1 := match (IntMap.find voter voterWeight) with
  |None => 0
  | Some a => a end in
 let voterWeight := IntMap.add voter (1)voterWeight in
-(create_Ballot voteCounts delegations votes voted voterWeight numProposals chairperson).
-Definition delegate (Ballot:Ballot) (to:Z)  := 
+((create_Ballot voteCounts delegations votes voted voterWeight numProposals chairperson), new_ether)end.
+Fixpoint delegate gas (Ballot:Ballot) (ether : EtherMap) (msg : Message)(to:Z)  := 
 let voteCounts := (voteCounts Ballot) in
 let delegations := (delegations Ballot) in
 let votes := (votes Ballot) in
@@ -79,9 +99,12 @@ let voted := (voted Ballot) in
 let voterWeight := (voterWeight Ballot) in
 let numProposals := (numProposals Ballot) in
 let chairperson := (chairperson Ballot) in
-let Ballot2 := Ballot in 
-if ((get_voted voted  (sender))) then ((create_Ballot voteCounts delegations votes voted voterWeight numProposals chairperson)) 
- else if (( eqb to sender)) then ((create_Ballot voteCounts delegations votes voted voterWeight numProposals chairperson)) 
+let new_ether := ether in 
+match gas with
+    | O => ((create_Ballot voteCounts delegations votes voted voterWeight numProposals chairperson), new_ether)
+ | S g => let new_gas := g in
+if ((get_voted voted  (sender))) then (((create_Ballot voteCounts delegations votes voted voterWeight numProposals chairperson), new_ether)) 
+ else if (( eqb to sender)) then (((create_Ballot voteCounts delegations votes voted voterWeight numProposals chairperson), new_ether)) 
  else let imap1 := match (IntMap.find sender voted) with
  |None => false
  | Some a => a end in
@@ -94,7 +117,7 @@ if ((get_voted voted  (to))) then (let imap1 := match (IntMap.find (get_votes vo
  |None => 0
  | Some a => a end in
 let voteCounts := IntMap.add (get_votes votes  (to)) (((get_voteCounts voteCounts  ((get_votes votes  (to)))) + (get_voterWeight voterWeight  (sender))))voteCounts in
-(create_Ballot voteCounts delegations votes voted voterWeight numProposals chairperson)) 
+((create_Ballot voteCounts delegations votes voted voterWeight numProposals chairperson), new_ether)) 
 else (let imap1 := match (IntMap.find to voterWeight) with
  |None => 0
  | Some a => a end in
@@ -103,9 +126,9 @@ let imap1 := match (IntMap.find sender voterWeight) with
  |None => 0
  | Some a => a end in
 let voterWeight := IntMap.add sender (0)voterWeight in
-(create_Ballot voteCounts delegations votes voted voterWeight numProposals chairperson))
-.
-Definition vote (Ballot:Ballot) (proposal:Z)  := 
+((create_Ballot voteCounts delegations votes voted voterWeight numProposals chairperson), new_ether))
+end.
+Fixpoint vote gas (Ballot:Ballot) (ether : EtherMap) (msg : Message)(proposal:Z)  := 
 let voteCounts := (voteCounts Ballot) in
 let delegations := (delegations Ballot) in
 let votes := (votes Ballot) in
@@ -113,8 +136,11 @@ let voted := (voted Ballot) in
 let voterWeight := (voterWeight Ballot) in
 let numProposals := (numProposals Ballot) in
 let chairperson := (chairperson Ballot) in
-let Ballot2 := Ballot in 
-if (( orb (get_voted voted  (sender)) ( ltb numProposals proposal))) then ((create_Ballot voteCounts delegations votes voted voterWeight numProposals chairperson)) 
+let new_ether := ether in 
+match gas with
+    | O => ((create_Ballot voteCounts delegations votes voted voterWeight numProposals chairperson), new_ether)
+ | S g => let new_gas := g in
+if (( orb (get_voted voted  (sender)) ( ltb numProposals proposal))) then (((create_Ballot voteCounts delegations votes voted voterWeight numProposals chairperson), new_ether)) 
  else let imap1 := match (IntMap.find sender voted) with
  |None => false
  | Some a => a end in
@@ -127,7 +153,7 @@ let imap1 := match (IntMap.find proposal voteCounts) with
  |None => 0
  | Some a => a end in
 let voteCounts := IntMap.add proposal (((get_voteCounts voteCounts  (proposal)) + (get_voterWeight voterWeight  (sender))))voteCounts in
-(create_Ballot voteCounts delegations votes voted voterWeight numProposals chairperson).
+((create_Ballot voteCounts delegations votes voted voterWeight numProposals chairperson), new_ether)end.
 Lemma plus_reg_r : forall (n m p : Z), n = m -> p+n= p+m.
 Proof.
   intros.
@@ -197,273 +223,4 @@ rewrite -> H0.
 symmetry.
 apply Zplus_0_r_reverse.
 Qed.
-
-
-Lemma extract_Sorted_0 : forall (a b : Z*Z) (l : list (Z * Z)),
-  Sorted.Sorted (IntMap.Raw.PX.ltk (elt:=Z)) (a::b::l) -> Sorted.Sorted (IntMap.Raw.PX.ltk (elt:=Z)) (b::l).
-Proof.
-  intros.
-  apply Sorted.Sorted_inv in H.
-  apply H.
-Qed. 
-
-Definition mapping_function_voterWeight ( x : Z * Z) := 
- (snd (x)).
-Fixpoint sum_voterWeight (maplist : list (Z * Z)) := 
- match maplist with
-    | nil => 0
-    | a::q => (mapping_function_voterWeight a) + (sum_voterWeight q)
-end.
-Lemma update_voterWeight : forall ( Ballot2 : Ballot ) (address : Z) (value : Z),
-      let balance_map := (voterWeight Ballot2) in
-      let original_value := match (IntMap.find address (voterWeight Ballot2)) with
-      | None => 0
-      | Some a => mapping_function_voterWeight(address, a) end in
-      let balance2 := sum_voterWeight (IntMap.elements (IntMap.add address value balance_map)) in
-      (sum_voterWeight (IntMap.elements balance_map)) + mapping_function_voterWeight(address, value) = balance2 + original_value.
-      Proof.
-      Opaque mapping_function_voterWeight.
-      intros.
-      case_eq (IntMap.find (elt := Z) address (voterWeight Ballot2)).
-      intro t0.
-      unfold balance2.
-      unfold sum_voterWeight.
-      simpl.
-      unfold get_voterWeight.
-      unfold balance_map.
-      destruct (voterWeight Ballot2).
-      intros.
-      simpl.
-      unfold IntMap.Raw.add.
-      remember (hd this) as a.
-      remember (tl this) as a_bis.
-      dependent induction this.
-      - assert (original_value = 0).
-      simpl in original_value.
-      auto.
-      rewrite -> H0.
-      simpl.
-      symmetry.
-      rewrite -> Z.add_comm.
-      simpl.
-      rewrite -> Z.add_comm.
-      simpl.
-      reflexivity.
-      - simpl.
-      destruct a as (z0, z1).
-      destruct (Z_as_OT.compare).
-      + simpl.
-      assert (IntMap.find (elt := Z) address {| IntMap.this := (z0, z1) :: this; IntMap.sorted := sorted |} = None).
-      unfold IntMap.find.
-      unfold IntMap.Raw.find.
-      simpl.
-      destruct Z_as_OT.compare.
-      reflexivity.
-      unfold Z_as_OT.lt in l.
-      unfold Z_as_OT.eq in e.
-      apply Z_as_OT.lt_not_eq in e.
-      contradiction.
-      apply l.
-      apply Z_as_OT.lt_trans with (x:=z0) (y:=address) (z:=z0) in l0.
-      apply Z_as_OT.lt_not_eq in l0.
-      compute in l0.
-      absurd (z0 = z0).
-      auto.
-      reflexivity.
-      apply l.
-      rewrite -> H0 in H.
-      discriminate.
-      + rewrite <- Z.add_comm.
-      symmetry.
-      rewrite <- Z.add_assoc.
-      apply plus_reg_r.
-      rewrite -> Z.add_comm.
-      assert (original_value = mapping_function_voterWeight (z0, z1)).
-      unfold original_value.
-      rewrite -> e.
-      unfold IntMap.find.
-      unfold IntMap.Raw.find.
-      simpl.
-      destruct Z_as_OT.compare.
-      apply Z_as_OT.lt_not_eq in l.
-      absurd (z0 <> z0).
-      auto.
-      apply l.
-      rewrite -> e.
-      reflexivity.
-      apply Z_as_OT.lt_not_eq in l.
-      absurd (z0 <> z0).
-      auto.
-      apply l.
-      rewrite -> H0.
-      reflexivity.
-      + rewrite <- Z.add_assoc.
-      symmetry.
-      rewrite <- Z.add_assoc.
-      apply plus_reg_r.
-      symmetry.
-      assert (Sorted (IntMap.Raw.PX.ltk (elt := Z)) this).
-      induction this.
-      auto.
-      apply extract_Sorted_0 with (a:=(z0, z1)).
-      apply sorted.
-      assert (original_value = match
-        IntMap.find (elt := Z) address {| IntMap.this := this; IntMap.sorted := H0 |} with
-        | Some a => mapping_function_voterWeight (address, a)
-        | None => 0
-        end).
-      unfold original_value.
-      unfold IntMap.find.
-      unfold IntMap.Raw.find.
-      simpl.
-      destruct Z_as_OT.compare.
-      apply Z_as_OT.lt_trans with (x:=address) (y:=z0) (z:=address) in l0.
-      absurd (address < address).
-      auto.
-      apply l0.
-      apply l.
-      rewrite -> e in l.
-      apply Z_as_OT.lt_not_eq in l.
-      absurd (z0 <> z0).
-      auto.
-      apply l.
-      reflexivity.
-      rewrite -> H1.
-      apply IHthis with (sorted := H0) (a := hd this) (a_bis := tl this) (t0:=t0).
-      unfold IntMap.find.
-      unfold IntMap.Raw.find.
-      simpl.
-      unfold IntMap.find in H.
-      unfold IntMap.Raw.find in H.
-      simpl in H.
-      destruct Z_as_OT.compare in H.
-      apply Z_as_OT.lt_trans with (x:=address) (y:=z0) (z:=address) in l0.
-      absurd (address < address).
-      auto.
-      apply l0.
-      apply l.
-      rewrite -> e in l.
-      apply Z_as_OT.lt_not_eq in l.
-      absurd (z0 <> z0).
-      auto.
-      apply l.
-      apply H.
-      reflexivity.
-      reflexivity.
-      - intros.
-      assert (original_value = 0).
-      unfold original_value.
-      rewrite -> H.
-      reflexivity.
-      rewrite -> H0.
-      unfold balance2.
-      unfold balance_map.
-      destruct (voterWeight Ballot2).
-      simpl.
-      dependent induction this.
-      simpl.
-      symmetry.
-      rewrite -> Z.add_comm.
-      simpl.
-      rewrite -> Z.add_comm.
-      simpl.
-      reflexivity.
-      unfold IntMap.Raw.add.
-      destruct a as (z, t0).
-      destruct Z_as_OT.compare.
-      unfold sum_voterWeight.
-      rewrite -> Z.add_comm.
-      symmetry.
-      rewrite <- Z.add_assoc.
-      apply plus_reg_r.
-      rewrite -> Z.add_comm.
-      simpl.
-      reflexivity.
-      simpl.
-      assert (original_value = mapping_function_voterWeight (z, t0)).
-      unfold original_value.
-      unfold IntMap.find.
-      unfold IntMap.Raw.find.
-      simpl.
-      destruct Z_as_OT.compare.
-      apply Z_as_OT.lt_not_eq in l.
-      rewrite -> e in l.
-      absurd (z <> z).
-      auto.
-      apply l.
-      rewrite -> e.
-      reflexivity.
-      rewrite -> e in l.
-      apply Z_as_OT.lt_not_eq in l.
-      absurd (z <> z).
-      auto.
-      apply l.
-      rewrite -> H0 in H1.
-      rewrite <- H1.
-      simpl.
-      symmetry.
-      rewrite <- Z.add_comm.
-      simpl.
-      rewrite <- Z.add_comm.
-      reflexivity.
-      unfold IntMap.Raw.add in IHthis.
-      unfold sum_voterWeight.
-      rewrite <- Z.add_assoc.
-      symmetry.
-      rewrite <- Z.add_assoc.
-      symmetry.
-      apply plus_reg_r.
-      unfold sum_voterWeight in IHthis.
-      assert (Sorted (IntMap.Raw.PX.ltk (elt := Z)) this).
-      induction this.
-      auto.
-      apply extract_Sorted_0 with (a:= (z, t0)).
-      apply sorted.
-      apply IHthis with (sorted := H1).
-      unfold IntMap.find.
-      unfold IntMap.Raw.find.
-      simpl.
-      unfold IntMap.find in H.
-      unfold IntMap.Raw.find in H.
-      simpl in H.
-      destruct Z_as_OT.compare in H.
-      apply Z_as_OT.lt_trans with (x:=z) (y:=address) (z:=z) in l.
-      absurd (z<z).
-      auto.
-      apply l.
-      apply l0.
-      discriminate.
-      apply H.
-      assert (IntMap.find (elt := Z) address {| IntMap.this := this; IntMap.sorted := H1 |} = None).
-      unfold IntMap.find.
-      unfold IntMap.Raw.find.
-      simpl.
-      unfold IntMap.find in H.
-      unfold IntMap.Raw.find in H.
-      simpl in H.
-      destruct Z_as_OT.compare in H.
-      apply Z_as_OT.lt_trans with (x:=z) (y:=address) (z:=z) in l.
-      absurd (z<z).
-      auto.
-      apply l.
-      apply l0.
-      discriminate.
-      apply H.
-      rewrite -> H2.
-      reflexivity.
-      Qed.
-Lemma preservation_vote_voterWeight : forall (Ballot : Ballot) (proposal:Z) , 
- let Ballot_2 := vote Ballot proposal in
- (sum_voterWeight (IntMap.elements (voterWeight Ballot))) = ( sum_voterWeight (IntMap.elements (voterWeight Ballot_2))).
-Admitted.
-
-Lemma preservation_delegate_voterWeight : forall (Ballot : Ballot) (to:Z) , 
- let Ballot_2 := delegate Ballot to in
- (sum_voterWeight (IntMap.elements (voterWeight Ballot))) = ( sum_voterWeight (IntMap.elements (voterWeight Ballot_2))).
-Admitted.
-
-Lemma preservation_giveRightToVote_voterWeight : forall (Ballot : Ballot) (voter:Z) , 
- let Ballot_2 := giveRightToVote Ballot voter in
- (sum_voterWeight (IntMap.elements (voterWeight Ballot))) = ( sum_voterWeight (IntMap.elements (voterWeight Ballot_2))).
-Admitted.
 
