Auction/Auction.v
@@ -8,103 +8,87 @@ Open Scope Z_scope.
 Include BinIntDef.Z.
 Module IntMap := FMapList.Make(Z_as_OT).
 Definition contract_addr := 0.
-
 Definition EtherMap := IntMap.t Z.
 
-Record Message := create_message {
-sender: Z;
-value: Z;
-}.
-
 Definition get_ether (addr : Z) map : Z :=
-  match (IntMap.find addr map) with
-  | None => 0
-  | Some a => a
-  end.
+    match (IntMap.find addr map) with
+    | None => 0
+    | Some a => a
+    end.
 
-Definition send addr value map := 
-  if (leb value (get_ether contract_addr map)) then 
-    (let map_bis := IntMap.add contract_addr ((get_ether contract_addr map) - value) map in
-    let map_bis := IntMap.add addr ((get_ether addr map_bis) + value) map_bis in
-    (true, map_bis))
-  else (false, map).
+Definition send addr value map :=
+    if (Z.leb value (get_ether contract_addr map)) then
+        (let map_bis := IntMap.add contract_addr ((get_ether contract_addr map) - value) map in
+        let map_bis := IntMap.add addr ((get_ether addr map_bis) + value) map_bis in
+        (true, map_bis))
+    else (false, map).
 
+Record Message := create_message {
+sender : Z;
+value : Z;
+}.
 Record Auction := create_Auction { 
 bids: IntMap.t (Z);
 isWinner: IntMap.t (bool);
 highestBid: Z;
 }.
-
+Definition get_bids (mapping : IntMap.t (Z) ) (a0 : Z) := 
+let m1:= match (IntMap.find a0 mapping)  with
+ | None => 0
+ | Some a => a end in 
+m1.
 Definition get_isWinner (mapping : IntMap.t (bool) ) (a0 : Z) := 
 let m1:= match (IntMap.find a0 mapping)  with
  | None => false
  | Some a => a end in 
 m1.
-
-Definition get_money (Auction : Auction) (ether : EtherMap) (msg: Message) :=
-  if (get_isWinner (isWinner Auction) (sender msg)) then 
-  (let (_, new_ether) := send (sender msg) (highestBid Auction) ether in
-    let isWinner := IntMap.add (sender msg) false (isWinner Auction) in
-    (create_Auction (bids Auction) isWinner (highestBid Auction), new_ether))
-  else (Auction, ether).
-
-Require Import Bool.
-
-Lemma test_send : forall (Auction : Auction) (ether : EtherMap) (msg: Message),
-  Is_true (get_isWinner (isWinner Auction) (sender msg)) -> Is_true (ltb 0 (highestBid Auction)) 
-  -> let (_, etherbis) := get_money Auction ether msg in Is_true (ltb (get_ether (sender msg) ether) (get_ether (sender msg) etherbis)).
-Proof.
-intros.
-unfold get_money.
-destruct (get_isWinner (isWinner Auction0) (sender msg)).
-* unfold send.
-  destruct (highestBid Auction0 <=?
-     get_ether contract_addr ether).
-  admit.
-  destruct (get_ether (sender msg) ether <? get_ether (sender msg) ether).
-  trivial.
-  (* This point is impossible : incorrect behaviour *)
-  admit.
-* contradiction.
-Admitted.
-
-
-Definition get_bids (mapping : IntMap.t (Z) ) (a0 : Z) : Z := 
-let m1:= match (IntMap.find a0 mapping)  with
- | None => 0
- | Some a => a end in 
-m1.
-
-Definition Auction_constructor (ether: EtherMap) (msg : Message):= 
+Fixpoint Auction_constructor(ether : EtherMap) (msg : Message) := 
 let bids := IntMap.empty (Z) in
 let isWinner := IntMap.empty (bool) in
 let highestBid := 0 in
+let new_ether := ether in
 let highestBid := 0 in 
 let imap1 := match (IntMap.find (sender msg) isWinner) with
  |None => false
  | Some a => a end in
 let isWinner := IntMap.add (sender msg) (true)isWinner in
-(create_Auction bids isWinner highestBid).
-
-Definition bid (Auction:Auction) (value:Z) (ether: EtherMap) (msg : Message) := 
+((create_Auction bids isWinner highestBid), new_ether).
+Fixpoint bid gas (Auction:Auction) (ether : EtherMap) (msg : Message)(value:Z)  := 
 let bids := (bids Auction) in
 let isWinner := (isWinner Auction) in
 let highestBid := (highestBid Auction) in
-let Auction2 := Auction in 
-if (( Z.leb value (get_bids bids  (sender msg)))) then (Auction) 
+let new_ether := ether in 
+match gas with
+    | O => ((create_Auction bids isWinner highestBid), new_ether)
+ | S g => let new_gas := g in
+if (( leb value (get_bids bids  ((sender msg))))) then ((Auction, ether)) 
 else (let imap1 := match (IntMap.find (sender msg) bids) with
  |None => 0
  | Some a => a end in
 let bids := IntMap.add (sender msg) (value)bids in
-if (( Z.leb highestBid value)) then (let highestBid := value in 
+if (( leb highestBid value)) then (let highestBid := value in 
 let imap1 := match (IntMap.find (sender msg) isWinner) with
  |None => false
  | Some a => a end in
 let isWinner := IntMap.add (sender msg) (true)isWinner in
-(create_Auction bids isWinner highestBid)) 
- else (create_Auction bids isWinner highestBid))
-.
-
+((create_Auction bids isWinner highestBid), new_ether)) 
+ else ((create_Auction bids isWinner highestBid), new_ether))
+end.
+Fixpoint get_money gas (Auction:Auction) (ether : EtherMap) (msg : Message) := 
+let bids := (bids Auction) in
+let isWinner := (isWinner Auction) in
+let highestBid := (highestBid Auction) in
+let new_ether := ether in 
+match gas with
+    | O => ((create_Auction bids isWinner highestBid), new_ether)
+ | S g => let new_gas := g in
+if ((get_isWinner isWinner  ((sender msg)))) then (let (_, new_ether) := send (sender msg)  (highestBid) new_ether in
+let imap1 := match (IntMap.find (sender msg) isWinner) with
+ |None => false
+ | Some a => a end in
+let isWinner := IntMap.add (sender msg) (false)isWinner in
+((create_Auction bids isWinner highestBid), new_ether)) 
+ else ((create_Auction bids isWinner highestBid), new_ether)end.
 Lemma plus_reg_r : forall (n m p : Z), n = m -> p+n= p+m.
 Proof.
   intros.
